\begin{displaymath}
\infer[({\rm L}\land)]{P \land \top \lra P}{
  \infer[({\rm L}\top)]{P, \top \lra P}{
    P \lra P  }
}
\end{displaymath}

\begin{displaymath}
\infer[({\rm R}\land)]{P \lra P \land \top}{
  P \lra P  &
  \infer[({\rm R}\top)]{P \lra \top}{}
}
\end{displaymath}

\begin{displaymath}
\infer[({\rm L}\lor)]{P \lor \bot \lra P}{
  P \lra P  &
  \infer[({\rm L}\bot)]{\bot \lra P}{}
}
\end{displaymath}

\begin{displaymath}
\infer[({\rm R}\lor)]{P \lra P \lor \bot}{
  \infer[({\rm R}\bot)]{P \lra P, \bot}{
    P \lra P  }
}
\end{displaymath}

\begin{displaymath}
\infer[({\rm R}\bot)]{P \land \bot \lra \bot}{
  \infer[({\rm L}\land)]{P \land \bot \lra }{
    \infer[({\rm L}\bot)]{P, \bot \lra }{}
  }
}
\end{displaymath}

\begin{displaymath}
\infer[({\rm L}\bot)]{\bot \lra P \land \bot}{}
\end{displaymath}

\begin{displaymath}
\infer[({\rm R}\top)]{P \lor \top \lra \top}{}
\end{displaymath}

\begin{displaymath}
\infer[({\rm L}\top)]{\top \lra P \lor \top}{
  \infer[({\rm R}\lor)]{ \lra P \lor \top}{
    \infer[({\rm R}\top)]{ \lra P, \top}{}
  }
}
\end{displaymath}

\begin{displaymath}
\infer[({\rm L}\land)]{P \land P \lra P}{
  P, P \lra P}
\end{displaymath}

\begin{displaymath}
\infer[({\rm R}\land)]{P \lra P \land P}{
  P \lra P  &
  P \lra P}
\end{displaymath}

\begin{displaymath}
\infer[({\rm L}\lor)]{P \lor P \lra P}{
  P \lra P  &
  P \lra P}
\end{displaymath}

\begin{displaymath}
\infer[({\rm R}\lor)]{P \lra P \lor P}{
  P \lra P, P}
\end{displaymath}

\begin{displaymath}
\infer[({\rm L}\land)]{P \land Q \lra Q \land P}{
  \infer[({\rm R}\land)]{P, Q \lra Q \land P}{
    P, Q \lra Q    &
    P, Q \lra P  }
}
\end{displaymath}

\begin{displaymath}
\infer[({\rm L}\land)]{Q \land P \lra P \land Q}{
  \infer[({\rm R}\land)]{Q, P \lra P \land Q}{
    Q, P \lra P    &
    Q, P \lra Q  }
}
\end{displaymath}

\begin{displaymath}
\infer[({\rm R}\lor)]{P \lor Q \lra Q \lor P}{
  \infer[({\rm L}\lor)]{P \lor Q \lra Q, P}{
    P \lra Q, P    &
    Q \lra Q, P  }
}
\end{displaymath}

\begin{displaymath}
\infer[({\rm R}\lor)]{Q \lor P \lra P \lor Q}{
  \infer[({\rm L}\lor)]{Q \lor P \lra P, Q}{
    Q \lra P, Q    &
    P \lra P, Q  }
}
\end{displaymath}

\begin{displaymath}
\infer[({\rm L}\land)]{P \land Q \lra P}{
  P, Q \lra P}
\end{displaymath}

\begin{displaymath}
\infer[({\rm L}\land)]{P \land Q \lra Q}{
  P, Q \lra Q}
\end{displaymath}

\begin{displaymath}
\infer[({\rm R}\lor)]{P \lra P \lor Q}{
  P \lra P, Q}
\end{displaymath}

\begin{displaymath}
\infer[({\rm R}\lor)]{Q \lra P \lor Q}{
  Q \lra P, Q}
\end{displaymath}

\begin{displaymath}
\infer[({\rm L}\land)]{P \land Q \land R \lra (P \land Q) \land R}{
  \infer[({\rm L}\land)]{P, Q \land R \lra (P \land Q) \land R}{
    \infer[({\rm R}\land)]{P, Q, R \lra (P \land Q) \land R}{
      \infer[({\rm R}\land)]{P, Q, R \lra P \land Q}{
        P, Q, R \lra P        &
        P, Q, R \lra Q      }
      &
      P, Q, R \lra R    }
  }
}
\end{displaymath}

\begin{displaymath}
\infer[({\rm L}\land)]{(P \land Q) \land R \lra P \land Q \land R}{
  \infer[({\rm L}\land)]{P \land Q, R \lra P \land Q \land R}{
    \infer[({\rm R}\land)]{P, Q, R \lra P \land Q \land R}{
      P, Q, R \lra P      &
      \infer[({\rm R}\land)]{P, Q, R \lra Q \land R}{
        P, Q, R \lra Q        &
        P, Q, R \lra R      }
    }
  }
}
\end{displaymath}

\begin{displaymath}
\infer[({\rm R}\lor)]{P \lor Q \lor R \lra (P \lor Q) \lor R}{
  \infer[({\rm R}\lor)]{P \lor Q \lor R \lra P \lor Q, R}{
    \infer[({\rm L}\lor)]{P \lor Q \lor R \lra P, Q, R}{
      P \lra P, Q, R      &
      \infer[({\rm L}\lor)]{Q \lor R \lra P, Q, R}{
        Q \lra P, Q, R        &
        R \lra P, Q, R      }
    }
  }
}
\end{displaymath}

\begin{displaymath}
\infer[({\rm R}\lor)]{(P \lor Q) \lor R \lra P \lor Q \lor R}{
  \infer[({\rm R}\lor)]{(P \lor Q) \lor R \lra P, Q \lor R}{
    \infer[({\rm L}\lor)]{(P \lor Q) \lor R \lra P, Q, R}{
      \infer[({\rm L}\lor)]{P \lor Q \lra P, Q, R}{
        P \lra P, Q, R        &
        Q \lra P, Q, R      }
      &
      R \lra P, Q, R    }
  }
}
\end{displaymath}

\begin{displaymath}
\infer[({\rm L}\land)]{P \land Q \lor R \lra (P \land Q) \lor P \land R}{
  \infer[({\rm R}\lor)]{P, Q \lor R \lra (P \land Q) \lor P \land R}{
    \infer[({\rm R}\land)]{P, Q \lor R \lra P \land Q, P \land R}{
      \infer[({\rm R}\land)]{P, Q \lor R \lra P, P \land R}{
        \infer[({\rm L}\lor)]{P, Q \lor R \lra P, P}{
          P, Q \lra P, P          &
          P, R \lra P, P        }
        &
        \infer[({\rm L}\lor)]{P, Q \lor R \lra P, R}{
          P, Q \lra P, R          &
          P, R \lra P, R        }
      }
      &
      \infer[({\rm R}\land)]{P, Q \lor R \lra Q, P \land R}{
        \infer[({\rm L}\lor)]{P, Q \lor R \lra Q, P}{
          P, Q \lra Q, P          &
          P, R \lra Q, P        }
        &
        \infer[({\rm L}\lor)]{P, Q \lor R \lra Q, R}{
          P, Q \lra Q, R          &
          P, R \lra Q, R        }
      }
    }
  }
}
\end{displaymath}

\begin{displaymath}
\infer[({\rm R}\land)]{(P \land Q) \lor P \land R \lra P \land Q \lor R}{
  \infer[({\rm L}\lor)]{(P \land Q) \lor P \land R \lra P}{
    \infer[({\rm L}\land)]{P \land Q \lra P}{
      P, Q \lra P    }
    &
    \infer[({\rm L}\land)]{P \land R \lra P}{
      P, R \lra P    }
  }
  &
  \infer[({\rm R}\lor)]{(P \land Q) \lor P \land R \lra Q \lor R}{
    \infer[({\rm L}\lor)]{(P \land Q) \lor P \land R \lra Q, R}{
      \infer[({\rm L}\land)]{P \land Q \lra Q, R}{
        P, Q \lra Q, R      }
      &
      \infer[({\rm L}\land)]{P \land R \lra Q, R}{
        P, R \lra Q, R      }
    }
  }
}
\end{displaymath}

\begin{displaymath}
\infer[({\rm R}\land)]{P \lor Q \land R \lra (P \lor Q) \land P \lor R}{
  \infer[({\rm R}\lor)]{P \lor Q \land R \lra P \lor Q}{
    \infer[({\rm L}\lor)]{P \lor Q \land R \lra P, Q}{
      P \lra P, Q      &
      \infer[({\rm L}\land)]{Q \land R \lra P, Q}{
        Q, R \lra P, Q      }
    }
  }
  &
  \infer[({\rm R}\lor)]{P \lor Q \land R \lra P \lor R}{
    \infer[({\rm L}\lor)]{P \lor Q \land R \lra P, R}{
      P \lra P, R      &
      \infer[({\rm L}\land)]{Q \land R \lra P, R}{
        Q, R \lra P, R      }
    }
  }
}
\end{displaymath}

\begin{displaymath}
\infer[({\rm L}\land)]{(P \lor Q) \land P \lor R \lra P \lor Q \land R}{
  \infer[({\rm R}\lor)]{P \lor Q, P \lor R \lra P \lor Q \land R}{
    \infer[({\rm R}\land)]{P \lor Q, P \lor R \lra P, Q \land R}{
      \infer[({\rm L}\lor)]{P \lor Q, P \lor R \lra P, Q}{
        \infer[({\rm L}\lor)]{P, P \lor R \lra P, Q}{
          P, P \lra P, Q          &
          P, R \lra P, Q        }
        &
        \infer[({\rm L}\lor)]{Q, P \lor R \lra P, Q}{
          Q, P \lra P, Q          &
          Q, R \lra P, Q        }
      }
      &
      \infer[({\rm L}\lor)]{P \lor Q, P \lor R \lra P, R}{
        \infer[({\rm L}\lor)]{P, P \lor R \lra P, R}{
          P, P \lra P, R          &
          P, R \lra P, R        }
        &
        \infer[({\rm L}\lor)]{Q, P \lor R \lra P, R}{
          Q, P \lra P, R          &
          Q, R \lra P, R        }
      }
    }
  }
}
\end{displaymath}

\begin{displaymath}
\infer[({\rm L}\land)]{P \land Q \lor R \lra (P \lor Q) \land P \lor R}{
  \infer[({\rm R}\land)]{P, Q \lor R \lra (P \lor Q) \land P \lor R}{
    \infer[({\rm R}\lor)]{P, Q \lor R \lra P \lor Q}{
      \infer[({\rm L}\lor)]{P, Q \lor R \lra P, Q}{
        P, Q \lra P, Q        &
        P, R \lra P, Q      }
    }
    &
    \infer[({\rm R}\lor)]{P, Q \lor R \lra P \lor R}{
      \infer[({\rm L}\lor)]{P, Q \lor R \lra P, R}{
        P, Q \lra P, R        &
        P, R \lra P, R      }
    }
  }
}
\end{displaymath}

\begin{displaymath}
\infer[({\rm R}\lor)]{(P \land Q) \lor P \land R \lra P \lor Q \land R}{
  \infer[({\rm R}\land)]{(P \land Q) \lor P \land R \lra P, Q \land R}{
    \infer[({\rm L}\lor)]{(P \land Q) \lor P \land R \lra P, Q}{
      \infer[({\rm L}\land)]{P \land Q \lra P, Q}{
        P, Q \lra P, Q      }
      &
      \infer[({\rm L}\land)]{P \land R \lra P, Q}{
        P, R \lra P, Q      }
    }
    &
    \infer[({\rm L}\lor)]{(P \land Q) \lor P \land R \lra P, R}{
      \infer[({\rm L}\land)]{P \land Q \lra P, R}{
        P, Q \lra P, R      }
      &
      \infer[({\rm L}\land)]{P \land R \lra P, R}{
        P, R \lra P, R      }
    }
  }
}
\end{displaymath}

\begin{displaymath}
\infer[({\rm L}\lnot)]{\lnot \lnot P \lra P}{
  \infer[({\rm R}\lnot)]{ \lra \lnot P, P}{
    P \lra P  }
}
\end{displaymath}

\begin{displaymath}
\infer[({\rm R}\lnot)]{P \lra \lnot \lnot P}{
  \infer[({\rm L}\lnot)]{\lnot P, P \lra }{
    P \lra P  }
}
\end{displaymath}

\begin{displaymath}
\infer[({\rm R}\bot)]{P \land \lnot P \lra \bot}{
  \infer[({\rm L}\land)]{P \land \lnot P \lra }{
    \infer[({\rm L}\lnot)]{P, \lnot P \lra }{
      P \lra P    }
  }
}
\end{displaymath}

\begin{displaymath}
\infer[({\rm L}\bot)]{\bot \lra P \land \lnot P}{}
\end{displaymath}

\begin{displaymath}
\infer[({\rm R}\top)]{P \lor \lnot P \lra \top}{}
\end{displaymath}

\begin{displaymath}
\infer[({\rm L}\top)]{\top \lra P \lor \lnot P}{
  \infer[({\rm R}\lor)]{ \lra P \lor \lnot P}{
    \infer[({\rm R}\lnot)]{ \lra P, \lnot P}{
      P \lra P    }
  }
}
\end{displaymath}

\begin{displaymath}
\infer[({\rm L}\lnot)]{\lnot (P \land Q) \lra \lnot P \lor \lnot Q}{
  \infer[({\rm R}\lor)]{ \lra P \land Q, \lnot P \lor \lnot Q}{
    \infer[({\rm R}\lnot)]{ \lra P \land Q, \lnot P, \lnot Q}{
      \infer[({\rm R}\lnot)]{P \lra P \land Q, \lnot Q}{
        \infer[({\rm R}\land)]{Q, P \lra P \land Q}{
          Q, P \lra P          &
          Q, P \lra Q        }
      }
    }
  }
}
\end{displaymath}

\begin{displaymath}
\infer[({\rm R}\lnot)]{\lnot P \lor \lnot Q \lra \lnot (P \land Q)}{
  \infer[({\rm L}\land)]{P \land Q, \lnot P \lor \lnot Q \lra }{
    \infer[({\rm L}\lor)]{P, Q, \lnot P \lor \lnot Q \lra }{
      \infer[({\rm L}\lnot)]{P, Q, \lnot P \lra }{
        P, Q \lra P      }
      &
      \infer[({\rm L}\lnot)]{P, Q, \lnot Q \lra }{
        P, Q \lra Q      }
    }
  }
}
\end{displaymath}

\begin{displaymath}
\infer[({\rm L}\lnot)]{\lnot (P \lor Q) \lra \lnot P \land \lnot Q}{
  \infer[({\rm R}\lor)]{ \lra P \lor Q, \lnot P \land \lnot Q}{
    \infer[({\rm R}\land)]{ \lra P, Q, \lnot P \land \lnot Q}{
      \infer[({\rm R}\lnot)]{ \lra P, Q, \lnot P}{
        P \lra P, Q      }
      &
      \infer[({\rm R}\lnot)]{ \lra P, Q, \lnot Q}{
        Q \lra P, Q      }
    }
  }
}
\end{displaymath}

\begin{displaymath}
\infer[({\rm R}\lnot)]{\lnot P \land \lnot Q \lra \lnot (P \lor Q)}{
  \infer[({\rm L}\land)]{P \lor Q, \lnot P \land \lnot Q \lra }{
    \infer[({\rm L}\lnot)]{P \lor Q, \lnot P, \lnot Q \lra }{
      \infer[({\rm L}\lnot)]{P \lor Q, \lnot Q \lra P}{
        \infer[({\rm L}\lor)]{P \lor Q \lra Q, P}{
          P \lra Q, P          &
          Q \lra Q, P        }
      }
    }
  }
}
\end{displaymath}

\begin{displaymath}
\infer[({\rm R}\lor)]{P \imp Q \lra \lnot P \lor Q}{
  \infer[({\rm R}\lnot)]{P \imp Q \lra \lnot P, Q}{
    \infer[({\rm L}\imp)]{P, P \imp Q \lra Q}{
      P \lra P, Q      &
      P, Q \lra Q    }
  }
}
\end{displaymath}

\begin{displaymath}
\infer[({\rm R}\imp)]{\lnot P \lor Q \lra P \imp Q}{
  \infer[({\rm L}\lor)]{P, \lnot P \lor Q \lra Q}{
    \infer[({\rm L}\lnot)]{P, \lnot P \lra Q}{
      P \lra P, Q    }
    &
    P, Q \lra Q  }
}
\end{displaymath}

\begin{displaymath}
\infer[({\rm L}\lnot)]{\lnot P \lra P \imp \bot}{
  \infer[({\rm R}\imp)]{ \lra P, P \imp \bot}{
    \infer[({\rm R}\bot)]{P \lra P, \bot}{
      P \lra P    }
  }
}
\end{displaymath}

\begin{displaymath}
\infer[({\rm R}\lnot)]{P \imp \bot \lra \lnot P}{
  \infer[({\rm L}\imp)]{P, P \imp \bot \lra }{
    P \lra P    &
    \infer[({\rm L}\bot)]{P, \bot \lra }{}
  }
}
\end{displaymath}

\begin{displaymath}
\infer[({\rm R}\imp)]{P \imp Q \lra \lnot Q \imp \lnot P}{
  \infer[({\rm L}\lnot)]{\lnot Q, P \imp Q \lra \lnot P}{
    \infer[({\rm R}\lnot)]{P \imp Q \lra Q, \lnot P}{
      \infer[({\rm L}\imp)]{P, P \imp Q \lra Q}{
        P \lra P, Q        &
        P, Q \lra Q      }
    }
  }
}
\end{displaymath}

\begin{displaymath}
\infer[({\rm R}\imp)]{\lnot Q \imp \lnot P \lra P \imp Q}{
  \infer[({\rm L}\imp)]{P, \lnot Q \imp \lnot P \lra Q}{
    \infer[({\rm R}\lnot)]{P \lra \lnot Q, Q}{
      Q, P \lra Q    }
    &
    \infer[({\rm L}\lnot)]{P, \lnot P \lra Q}{
      P \lra P, Q    }
  }
}
\end{displaymath}

\begin{displaymath}
\infer[({\rm R}\imp)]{P \imp Q \imp R \lra Q \imp P \imp R}{
  \infer[({\rm R}\imp)]{Q, P \imp Q \imp R \lra P \imp R}{
    \infer[({\rm L}\imp)]{P, Q, P \imp Q \imp R \lra R}{
      P, Q \lra P, R      &
      \infer[({\rm L}\imp)]{P, Q, Q \imp R \lra R}{
        P, Q \lra Q, R        &
        P, Q, R \lra R      }
    }
  }
}
\end{displaymath}

\begin{displaymath}
\infer[({\rm R}\imp)]{Q \imp P \imp R \lra P \imp Q \imp R}{
  \infer[({\rm R}\imp)]{P, Q \imp P \imp R \lra Q \imp R}{
    \infer[({\rm L}\imp)]{Q, P, Q \imp P \imp R \lra R}{
      Q, P \lra Q, R      &
      \infer[({\rm L}\imp)]{Q, P, P \imp R \lra R}{
        Q, P \lra P, R        &
        Q, P, R \lra R      }
    }
  }
}
\end{displaymath}

\begin{displaymath}
\infer[({\rm R}\imp)]{P \imp Q \imp R \lra P \land Q \imp R}{
  \infer[({\rm L}\land)]{P \land Q, P \imp Q \imp R \lra R}{
    \infer[({\rm L}\imp)]{P, Q, P \imp Q \imp R \lra R}{
      P, Q \lra P, R      &
      \infer[({\rm L}\imp)]{P, Q, Q \imp R \lra R}{
        P, Q \lra Q, R        &
        P, Q, R \lra R      }
    }
  }
}
\end{displaymath}

\begin{displaymath}
\infer[({\rm R}\imp)]{P \land Q \imp R \lra P \imp Q \imp R}{
  \infer[({\rm R}\imp)]{P, P \land Q \imp R \lra Q \imp R}{
    \infer[({\rm L}\imp)]{Q, P, P \land Q \imp R \lra R}{
      \infer[({\rm R}\land)]{Q, P \lra P \land Q, R}{
        Q, P \lra P, R        &
        Q, P \lra Q, R      }
      &
      Q, P, R \lra R    }
  }
}
\end{displaymath}

\begin{displaymath}
\infer[({\rm L}\land)]{(P \imp Q) \land (P \imp R) \lra P \imp Q \land R}{
  \infer[({\rm R}\imp)]{P \imp Q, P \imp R \lra P \imp Q \land R}{
    \infer[({\rm R}\land)]{P, P \imp Q, P \imp R \lra Q \land R}{
      \infer[({\rm L}\imp)]{P, P \imp Q, P \imp R \lra Q}{
        \infer[({\rm L}\imp)]{P, P \imp R \lra P, Q}{
          P \lra P, P, Q          &
          P, R \lra P, Q        }
        &
        \infer[({\rm L}\imp)]{P, Q, P \imp R \lra Q}{
          P, Q \lra P, Q          &
          P, Q, R \lra Q        }
      }
      &
      \infer[({\rm L}\imp)]{P, P \imp Q, P \imp R \lra R}{
        \infer[({\rm L}\imp)]{P, P \imp R \lra P, R}{
          P \lra P, P, R          &
          P, R \lra P, R        }
        &
        \infer[({\rm L}\imp)]{P, Q, P \imp R \lra R}{
          P, Q \lra P, R          &
          P, Q, R \lra R        }
      }
    }
  }
}
\end{displaymath}

\begin{displaymath}
\infer[({\rm R}\land)]{P \imp Q \land R \lra (P \imp Q) \land (P \imp R)}{
  \infer[({\rm R}\imp)]{P \imp Q \land R \lra P \imp Q}{
    \infer[({\rm L}\imp)]{P, P \imp Q \land R \lra Q}{
      P \lra P, Q      &
      \infer[({\rm L}\land)]{P, Q \land R \lra Q}{
        P, Q, R \lra Q      }
    }
  }
  &
  \infer[({\rm R}\imp)]{P \imp Q \land R \lra P \imp R}{
    \infer[({\rm L}\imp)]{P, P \imp Q \land R \lra R}{
      P \lra P, R      &
      \infer[({\rm L}\land)]{P, Q \land R \lra R}{
        P, Q, R \lra R      }
    }
  }
}
\end{displaymath}

\begin{displaymath}
\infer[({\rm L}\land)]{(P \imp R) \land (Q \imp R) \lra P \lor Q \imp R}{
  \infer[({\rm R}\imp)]{P \imp R, Q \imp R \lra P \lor Q \imp R}{
    \infer[({\rm L}\lor)]{P \lor Q, P \imp R, Q \imp R \lra R}{
      \infer[({\rm L}\imp)]{P, P \imp R, Q \imp R \lra R}{
        \infer[({\rm L}\imp)]{P, Q \imp R \lra P, R}{
          P \lra Q, P, R          &
          P, R \lra P, R        }
        &
        \infer[({\rm L}\imp)]{P, R, Q \imp R \lra R}{
          P, R \lra Q, R          &
          P, R, R \lra R        }
      }
      &
      \infer[({\rm L}\imp)]{Q, P \imp R, Q \imp R \lra R}{
        \infer[({\rm L}\imp)]{Q, Q \imp R \lra P, R}{
          Q \lra Q, P, R          &
          Q, R \lra P, R        }
        &
        \infer[({\rm L}\imp)]{Q, R, Q \imp R \lra R}{
          Q, R \lra Q, R          &
          Q, R, R \lra R        }
      }
    }
  }
}
\end{displaymath}

\begin{displaymath}
\infer[({\rm R}\land)]{P \lor Q \imp R \lra (P \imp R) \land (Q \imp R)}{
  \infer[({\rm R}\imp)]{P \lor Q \imp R \lra P \imp R}{
    \infer[({\rm L}\imp)]{P, P \lor Q \imp R \lra R}{
      \infer[({\rm R}\lor)]{P \lra P \lor Q, R}{
        P \lra P, Q, R      }
      &
      P, R \lra R    }
  }
  &
  \infer[({\rm R}\imp)]{P \lor Q \imp R \lra Q \imp R}{
    \infer[({\rm L}\imp)]{Q, P \lor Q \imp R \lra R}{
      \infer[({\rm R}\lor)]{Q \lra P \lor Q, R}{
        Q \lra P, Q, R      }
      &
      Q, R \lra R    }
  }
}
\end{displaymath}

\begin{displaymath}
\infer[({\rm R}\imp)]{P \imp Q, Q \imp R \lra P \imp R}{
  \infer[({\rm L}\imp)]{P, P \imp Q, Q \imp R \lra R}{
    \infer[({\rm L}\imp)]{P, Q \imp R \lra P, R}{
      P \lra Q, P, R      &
      P, R \lra P, R    }
    &
    \infer[({\rm L}\imp)]{P, Q, Q \imp R \lra R}{
      P, Q \lra Q, R      &
      P, Q, R \lra R    }
  }
}
\end{displaymath}

\begin{displaymath}
\infer[({\rm R}\imp)]{ \lra P \imp Q \imp P}{
  \infer[({\rm R}\imp)]{P \lra Q \imp P}{
    Q, P \lra P  }
}
\end{displaymath}

\begin{displaymath}
\infer[({\rm R}\imp)]{ \lra (P \imp Q \imp R) \imp (P \imp Q) \imp P \imp R}{
  \infer[({\rm R}\imp)]{P \imp Q \imp R \lra (P \imp Q) \imp P \imp R}{
    \infer[({\rm R}\imp)]{P \imp Q, P \imp Q \imp R \lra P \imp R}{
      \infer[({\rm L}\imp)]{P, P \imp Q, P \imp Q \imp R \lra R}{
        \infer[({\rm L}\imp)]{P, P \imp Q \imp R \lra P, R}{
          P \lra P, P, R          &
          \infer[({\rm L}\imp)]{P, Q \imp R \lra P, R}{
            P \lra Q, P, R            &
            P, R \lra P, R          }
        }
        &
        \infer[({\rm L}\imp)]{P, Q, P \imp Q \imp R \lra R}{
          P, Q \lra P, R          &
          \infer[({\rm L}\imp)]{P, Q, Q \imp R \lra R}{
            P, Q \lra Q, R            &
            P, Q, R \lra R          }
        }
      }
    }
  }
}
\end{displaymath}

\begin{displaymath}
\infer[({\rm R}\imp)]{ \lra (P \imp \lnot Q) \imp (P \imp Q) \imp \lnot P}{
  \infer[({\rm R}\imp)]{P \imp \lnot Q \lra (P \imp Q) \imp \lnot P}{
    \infer[({\rm R}\lnot)]{P \imp Q, P \imp \lnot Q \lra \lnot P}{
      \infer[({\rm L}\imp)]{P, P \imp Q, P \imp \lnot Q \lra }{
        \infer[({\rm L}\imp)]{P, P \imp \lnot Q \lra P}{
          P \lra P, P          &
          \infer[({\rm L}\lnot)]{P, \lnot Q \lra P}{
            P \lra Q, P          }
        }
        &
        \infer[({\rm L}\imp)]{P, Q, P \imp \lnot Q \lra }{
          P, Q \lra P          &
          \infer[({\rm L}\lnot)]{P, Q, \lnot Q \lra }{
            P, Q \lra Q          }
        }
      }
    }
  }
}
\end{displaymath}

\begin{displaymath}
\infer[({\rm R}\imp)]{ \lra (\lnot P \imp \lnot Q) \imp (\lnot P \imp Q) \imp P}{
  \infer[({\rm R}\imp)]{\lnot P \imp \lnot Q \lra (\lnot P \imp Q) \imp P}{
    \infer[({\rm L}\imp)]{\lnot P \imp Q, \lnot P \imp \lnot Q \lra P}{
      \infer[({\rm R}\lnot)]{\lnot P \imp \lnot Q \lra \lnot P, P}{
        \infer[({\rm L}\imp)]{P, \lnot P \imp \lnot Q \lra P}{
          \infer[({\rm R}\lnot)]{P \lra \lnot P, P}{
            P, P \lra P          }
          &
          \infer[({\rm L}\lnot)]{P, \lnot Q \lra P}{
            P \lra Q, P          }
        }
      }
      &
      \infer[({\rm L}\imp)]{Q, \lnot P \imp \lnot Q \lra P}{
        \infer[({\rm R}\lnot)]{Q \lra \lnot P, P}{
          P, Q \lra P        }
        &
        \infer[({\rm L}\lnot)]{Q, \lnot Q \lra P}{
          Q \lra Q, P        }
      }
    }
  }
}
\end{displaymath}

\begin{displaymath}
\infer[({\rm R}\imp)]{ \lra P \land (P \imp Q) \land (P \land Q \imp S) \imp S}{
  \infer[({\rm L}\land)]{P \land (P \imp Q) \land (P \land Q \imp S) \lra S}{
    \infer[({\rm L}\land)]{P, (P \imp Q) \land (P \land Q \imp S) \lra S}{
      \infer[({\rm L}\imp)]{P, P \imp Q, P \land Q \imp S \lra S}{
        \infer[({\rm L}\imp)]{P, P \land Q \imp S \lra P, S}{
          \infer[({\rm R}\land)]{P \lra P \land Q, P, S}{
            P \lra P, P, S            &
            P \lra Q, P, S          }
          &
          P, S \lra P, S        }
        &
        \infer[({\rm L}\imp)]{P, Q, P \land Q \imp S \lra S}{
          \infer[({\rm R}\land)]{P, Q \lra P \land Q, S}{
            P, Q \lra P, S            &
            P, Q \lra Q, S          }
          &
          P, Q, S \lra S        }
      }
    }
  }
}
\end{displaymath}

\begin{displaymath}
\infer[({\rm R}\lor)]{ \lra P \lor (P \imp Q)}{
  \infer[({\rm R}\imp)]{ \lra P, P \imp Q}{
    P \lra P, Q  }
}
\end{displaymath}

\begin{displaymath}
\infer[({\rm R}\imp)]{ \lra ((P \imp Q) \imp P) \imp P}{
  \infer[({\rm L}\imp)]{(P \imp Q) \imp P \lra P}{
    \infer[({\rm R}\imp)]{ \lra P \imp Q, P}{
      P \lra Q, P    }
    &
    P \lra P  }
}
\end{displaymath}

\begin{displaymath}
\infer[({\rm R}\land)]{\forall x.P(x) \lra P(a) \land P(b)}{
  \infer[({\rm L}\forall)]{\forall x.P(x) \lra P(a)}{
    P(a), \forall x.P(x) \lra P(a)  }
  &
  \infer[({\rm L}\forall)]{\forall x.P(x) \lra P(b)}{
    P(b), \forall x.P(x) \lra P(b)  }
}
\end{displaymath}

\begin{displaymath}
\infer[({\rm L}\lor)]{P(a) \lor P(b) \lra \exists x.P(x)}{
  \infer[({\rm R}\exists)]{P(a) \lra \exists x.P(x)}{
    P(a) \lra P(a), \exists x.P(x)  }
  &
  \infer[({\rm R}\exists)]{P(b) \lra \exists x.P(x)}{
    P(b) \lra P(b), \exists x.P(x)  }
}
\end{displaymath}

\begin{displaymath}
\infer[({\rm L}\forall)]{\forall x.\forall x.P(x) \lra \forall x.P(x)}{
  \forall x.P(x), \forall x.\forall x.P(x) \lra \forall x.P(x)}
\end{displaymath}

\begin{displaymath}
\infer[({\rm R}\forall)]{\forall x.P(x) \lra \forall x.\forall x.P(x)}{
  \infer[({\rm R}\forall)]{\forall x.P(x) \lra \forall y.P(y)}{
    \infer[({\rm L}\forall)]{\forall x.P(x) \lra P(z)}{
      P(z), \forall x.P(x) \lra P(z)    }
  }
}
\end{displaymath}

\begin{displaymath}
\infer[({\rm L}\exists)]{\exists x.\exists x.P(x) \lra \exists x.P(x)}{
  \infer[({\rm L}\exists)]{\exists y.P(y) \lra \exists x.P(x)}{
    \infer[({\rm R}\exists)]{P(z) \lra \exists x.P(x)}{
      P(z) \lra P(z), \exists x.P(x)    }
  }
}
\end{displaymath}

\begin{displaymath}
\infer[({\rm R}\exists)]{\exists x.P(x) \lra \exists x.\exists x.P(x)}{
  \exists x.P(x) \lra \exists x.P(x), \exists x.\exists x.P(x)}
\end{displaymath}

\begin{displaymath}
\infer[({\rm R}\land)]{\forall x.P(x) \land Q(x) \lra (\forall x.P(x)) \land (\forall x.Q(x))}{
  \infer[({\rm R}\forall)]{\forall x.P(x) \land Q(x) \lra \forall x.P(x)}{
    \infer[({\rm L}\forall)]{\forall x.P(x) \land Q(x) \lra P(y)}{
      \infer[({\rm L}\land)]{P(y) \land Q(y), \forall x.P(x) \land Q(x) \lra P(y)}{
        P(y), Q(y), \forall x.P(x) \land Q(x) \lra P(y)      }
    }
  }
  &
  \infer[({\rm R}\forall)]{\forall x.P(x) \land Q(x) \lra \forall x.Q(x)}{
    \infer[({\rm L}\forall)]{\forall x.P(x) \land Q(x) \lra Q(z)}{
      \infer[({\rm L}\land)]{P(z) \land Q(z), \forall x.P(x) \land Q(x) \lra Q(z)}{
        P(z), Q(z), \forall x.P(x) \land Q(x) \lra Q(z)      }
    }
  }
}
\end{displaymath}

\begin{displaymath}
\infer[({\rm L}\land)]{(\forall x.P(x)) \land (\forall x.Q(x)) \lra \forall x.P(x) \land Q(x)}{
  \infer[({\rm R}\forall)]{\forall x.P(x), \forall x.Q(x) \lra \forall x.P(x) \land Q(x)}{
    \infer[({\rm R}\land)]{\forall x.P(x), \forall x.Q(x) \lra P(y) \land Q(y)}{
      \infer[({\rm L}\forall)]{\forall x.P(x), \forall x.Q(x) \lra P(y)}{
        P(y), \forall x.P(x), \forall x.Q(x) \lra P(y)      }
      &
      \infer[({\rm L}\forall)]{\forall x.P(x), \forall x.Q(x) \lra Q(y)}{
        \forall x.P(x), Q(y), \forall x.Q(x) \lra Q(y)      }
    }
  }
}
\end{displaymath}

\begin{displaymath}
\infer[({\rm R}\lor)]{\exists x.P(x) \lor Q(x) \lra (\exists x.P(x)) \lor (\exists x.Q(x))}{
  \infer[({\rm L}\exists)]{\exists x.P(x) \lor Q(x) \lra \exists x.P(x), \exists x.Q(x)}{
    \infer[({\rm L}\lor)]{P(y) \lor Q(y) \lra \exists x.P(x), \exists x.Q(x)}{
      \infer[({\rm R}\exists)]{P(y) \lra \exists x.P(x), \exists x.Q(x)}{
        P(y) \lra P(y), \exists x.P(x), \exists x.Q(x)      }
      &
      \infer[({\rm R}\exists)]{Q(y) \lra \exists x.P(x), \exists x.Q(x)}{
        Q(y) \lra \exists x.P(x), Q(y), \exists x.Q(x)      }
    }
  }
}
\end{displaymath}

\begin{displaymath}
\infer[({\rm L}\lor)]{(\exists x.P(x)) \lor (\exists x.Q(x)) \lra \exists x.P(x) \lor Q(x)}{
  \infer[({\rm L}\exists)]{\exists x.P(x) \lra \exists x.P(x) \lor Q(x)}{
    \infer[({\rm R}\exists)]{P(y) \lra \exists x.P(x) \lor Q(x)}{
      \infer[({\rm R}\lor)]{P(y) \lra P(y) \lor Q(y), \exists x.P(x) \lor Q(x)}{
        P(y) \lra P(y), Q(y), \exists x.P(x) \lor Q(x)      }
    }
  }
  &
  \infer[({\rm L}\exists)]{\exists x.Q(x) \lra \exists x.P(x) \lor Q(x)}{
    \infer[({\rm R}\exists)]{Q(z) \lra \exists x.P(x) \lor Q(x)}{
      \infer[({\rm R}\lor)]{Q(z) \lra P(z) \lor Q(z), \exists x.P(x) \lor Q(x)}{
        Q(z) \lra P(z), Q(z), \exists x.P(x) \lor Q(x)      }
    }
  }
}
\end{displaymath}

\begin{displaymath}
\infer[({\rm L}\lnot)]{\lnot (\forall x.P(x)) \lra \exists x.\lnot P(x)}{
  \infer[({\rm R}\forall)]{ \lra \forall x.P(x), \exists x.\lnot P(x)}{
    \infer[({\rm R}\exists)]{ \lra P(y), \exists x.\lnot P(x)}{
      \infer[({\rm R}\lnot)]{ \lra P(y), \lnot P(y), \exists x.\lnot P(x)}{
        P(y) \lra P(y), \exists x.\lnot P(x)      }
    }
  }
}
\end{displaymath}

\begin{displaymath}
\infer[({\rm R}\lnot)]{\exists x.\lnot P(x) \lra \lnot (\forall x.P(x))}{
  \infer[({\rm L}\exists)]{\forall x.P(x), \exists x.\lnot P(x) \lra }{
    \infer[({\rm L}\lnot)]{\forall x.P(x), \lnot P(y) \lra }{
      \infer[({\rm L}\forall)]{\forall x.P(x) \lra P(y)}{
        P(y), \forall x.P(x) \lra P(y)      }
    }
  }
}
\end{displaymath}

\begin{displaymath}
\infer[({\rm L}\lnot)]{\lnot (\exists x.P(x)) \lra \forall x.\lnot P(x)}{
  \infer[({\rm R}\forall)]{ \lra \exists x.P(x), \forall x.\lnot P(x)}{
    \infer[({\rm R}\lnot)]{ \lra \exists x.P(x), \lnot P(y)}{
      \infer[({\rm R}\exists)]{P(y) \lra \exists x.P(x)}{
        P(y) \lra P(y), \exists x.P(x)      }
    }
  }
}
\end{displaymath}

\begin{displaymath}
\infer[({\rm R}\lnot)]{\forall x.\lnot P(x) \lra \lnot (\exists x.P(x))}{
  \infer[({\rm L}\exists)]{\exists x.P(x), \forall x.\lnot P(x) \lra }{
    \infer[({\rm L}\forall)]{P(y), \forall x.\lnot P(x) \lra }{
      \infer[({\rm L}\lnot)]{P(y), \lnot P(y), \forall x.\lnot P(x) \lra }{
        P(y), \forall x.\lnot P(x) \lra P(y)      }
    }
  }
}
\end{displaymath}

\begin{displaymath}
\infer[({\rm L}\lnot)]{\lnot (\forall x.P(x) \imp Q(x)) \lra \exists x.P(x) \land \lnot Q(x)}{
  \infer[({\rm R}\forall)]{ \lra \forall x.P(x) \imp Q(x), \exists x.P(x) \land \lnot Q(x)}{
    \infer[({\rm R}\imp)]{ \lra P(y) \imp Q(y), \exists x.P(x) \land \lnot Q(x)}{
      \infer[({\rm R}\exists)]{P(y) \lra Q(y), \exists x.P(x) \land \lnot Q(x)}{
        \infer[({\rm R}\land)]{P(y) \lra Q(y), P(y) \land \lnot Q(y), \exists x.P(x) \land \lnot Q(x)}{
          P(y) \lra Q(y), P(y), \exists x.P(x) \land \lnot Q(x)          &
          \infer[({\rm R}\lnot)]{P(y) \lra Q(y), \lnot Q(y), \exists x.P(x) \land \lnot Q(x)}{
            Q(y), P(y) \lra Q(y), \exists x.P(x) \land \lnot Q(x)          }
        }
      }
    }
  }
}
\end{displaymath}

\begin{displaymath}
\infer[({\rm R}\lnot)]{\exists x.P(x) \land \lnot Q(x) \lra \lnot (\forall x.P(x) \imp Q(x))}{
  \infer[({\rm L}\exists)]{\forall x.P(x) \imp Q(x), \exists x.P(x) \land \lnot Q(x) \lra }{
    \infer[({\rm L}\land)]{\forall x.P(x) \imp Q(x), P(y) \land \lnot Q(y) \lra }{
      \infer[({\rm L}\lnot)]{\forall x.P(x) \imp Q(x), P(y), \lnot Q(y) \lra }{
        \infer[({\rm L}\forall)]{\forall x.P(x) \imp Q(x), P(y) \lra Q(y)}{
          \infer[({\rm L}\imp)]{P(y) \imp Q(y), \forall x.P(x) \imp Q(x), P(y) \lra Q(y)}{
            \forall x.P(x) \imp Q(x), P(y) \lra P(y), Q(y)            &
            Q(y), \forall x.P(x) \imp Q(x), P(y) \lra Q(y)          }
        }
      }
    }
  }
}
\end{displaymath}

\begin{displaymath}
\infer[({\rm L}\lnot)]{\lnot (\exists x.P(x) \land Q(x)) \lra \forall x.P(x) \imp \lnot Q(x)}{
  \infer[({\rm R}\forall)]{ \lra \exists x.P(x) \land Q(x), \forall x.P(x) \imp \lnot Q(x)}{
    \infer[({\rm R}\imp)]{ \lra \exists x.P(x) \land Q(x), P(y) \imp \lnot Q(y)}{
      \infer[({\rm R}\lnot)]{P(y) \lra \exists x.P(x) \land Q(x), \lnot Q(y)}{
        \infer[({\rm R}\exists)]{Q(y), P(y) \lra \exists x.P(x) \land Q(x)}{
          \infer[({\rm R}\land)]{Q(y), P(y) \lra P(y) \land Q(y), \exists x.P(x) \land Q(x)}{
            Q(y), P(y) \lra P(y), \exists x.P(x) \land Q(x)            &
            Q(y), P(y) \lra Q(y), \exists x.P(x) \land Q(x)          }
        }
      }
    }
  }
}
\end{displaymath}

\begin{displaymath}
\infer[({\rm R}\lnot)]{\forall x.P(x) \imp \lnot Q(x) \lra \lnot (\exists x.P(x) \land Q(x))}{
  \infer[({\rm L}\exists)]{\exists x.P(x) \land Q(x), \forall x.P(x) \imp \lnot Q(x) \lra }{
    \infer[({\rm L}\land)]{P(y) \land Q(y), \forall x.P(x) \imp \lnot Q(x) \lra }{
      \infer[({\rm L}\forall)]{P(y), Q(y), \forall x.P(x) \imp \lnot Q(x) \lra }{
        \infer[({\rm L}\imp)]{P(y), Q(y), P(y) \imp \lnot Q(y), \forall x.P(x) \imp \lnot Q(x) \lra }{
          P(y), Q(y), \forall x.P(x) \imp \lnot Q(x) \lra P(y)          &
          \infer[({\rm L}\lnot)]{P(y), Q(y), \lnot Q(y), \forall x.P(x) \imp \lnot Q(x) \lra }{
            P(y), Q(y), \forall x.P(x) \imp \lnot Q(x) \lra Q(y)          }
        }
      }
    }
  }
}
\end{displaymath}

\begin{displaymath}
\infer[({\rm L}\forall)]{\forall x.P(x) \lra \exists x.P(x)}{
  \infer[({\rm R}\exists)]{P(y), \forall x.P(x) \lra \exists x.P(x)}{
    P(y), \forall x.P(x) \lra P(y), \exists x.P(x)  }
}
\end{displaymath}

\begin{displaymath}
\infer[({\rm R}\exists)]{ \lra \exists x.\forall y.P(y) \imp P(x)}{
  \infer[({\rm R}\forall)]{ \lra \forall y.P(y) \imp P(z), \exists x.\forall y.P(y) \imp P(x)}{
    \infer[({\rm R}\imp)]{ \lra P(x_{1}) \imp P(z), \exists x.\forall y.P(y) \imp P(x)}{
      \infer[({\rm R}\exists)]{P(x_{1}) \lra P(z), \exists x.\forall y.P(y) \imp P(x)}{
        \infer[({\rm R}\forall)]{P(x_{1}) \lra P(z), \forall y.P(y) \imp P(x_{1}), \exists x.\forall y.P(y) \imp P(x)}{
          \infer[({\rm R}\imp)]{P(x_{1}) \lra P(z), P(y_{1}) \imp P(x_{1}), \exists x.\forall y.P(y) \imp P(x)}{
            P(y_{1}), P(x_{1}) \lra P(z), P(x_{1}), \exists x.\forall y.P(y) \imp P(x)          }
        }
      }
    }
  }
}
\end{displaymath}

\begin{displaymath}
\infer[({\rm R}\forall)]{\exists x.\forall y.P(x,y) \lra \forall y.\exists x.P(x,y)}{
  \infer[({\rm L}\exists)]{\exists x.\forall y.P(x,y) \lra \exists x.P(x,z)}{
    \infer[({\rm L}\forall)]{\forall y.P(x_{1},y) \lra \exists x.P(x,z)}{
      \infer[({\rm R}\exists)]{P(x_{1},z), \forall y.P(x_{1},y) \lra \exists x.P(x,z)}{
        P(x_{1},z), \forall y.P(x_{1},y) \lra P(x_{1},z), \exists x.P(x,z)      }
    }
  }
}
\end{displaymath}

\begin{displaymath}
\infer[({\rm R}\imp)]{ \lra (P(a) \land P(b) \imp Q) \imp (\exists x.P(x) \imp Q)}{
  \infer[({\rm L}\imp)]{P(a) \land P(b) \imp Q \lra \exists x.P(x) \imp Q}{
    \infer[({\rm R}\land)]{ \lra P(a) \land P(b), \exists x.P(x) \imp Q}{
      \infer[({\rm R}\exists)]{ \lra P(a), \exists x.P(x) \imp Q}{
        \infer[({\rm R}\imp)]{ \lra P(a), P(a) \imp Q, \exists x.P(x) \imp Q}{
          P(a) \lra P(a), Q, \exists x.P(x) \imp Q        }
      }
      &
      \infer[({\rm R}\exists)]{ \lra P(b), \exists x.P(x) \imp Q}{
        \infer[({\rm R}\imp)]{ \lra P(b), P(b) \imp Q, \exists x.P(x) \imp Q}{
          P(b) \lra P(b), Q, \exists x.P(x) \imp Q        }
      }
    }
    &
    \infer[({\rm R}\exists)]{Q \lra \exists x.P(x) \imp Q}{
      \infer[({\rm R}\imp)]{Q \lra P(y) \imp Q, \exists x.P(x) \imp Q}{
        P(y), Q \lra Q, \exists x.P(x) \imp Q      }
    }
  }
}
\end{displaymath}

\begin{displaymath}
\infer[({\rm L}\forall)]{N(0), \forall x.N(x) \imp N(s(x)) \lra N(s(s(0)))}{
  \infer[({\rm L}\imp)]{N(0), N(0) \imp N(s(0)), \forall x.N(x) \imp N(s(x)) \lra N(s(s(0)))}{
    N(0), \forall x.N(x) \imp N(s(x)) \lra N(0), N(s(s(0)))    &
    \infer[({\rm L}\forall)]{N(0), N(s(0)), \forall x.N(x) \imp N(s(x)) \lra N(s(s(0)))}{
      \infer[({\rm L}\imp)]{N(0), N(s(0)), N(s(0)) \imp N(s(s(0))), \forall x.N(x) \imp N(s(x)) \lra N(s(s(0)))}{
        N(0), N(s(0)), \forall x.N(x) \imp N(s(x)) \lra N(s(0)), N(s(s(0)))        &
        N(0), N(s(0)), N(s(s(0))), \forall x.N(x) \imp N(s(x)) \lra N(s(s(0)))      }
    }
  }
}
\end{displaymath}

